iso_dh/shared.v
@@ -32,7 +32,7 @@ Section Verif.
 Context `{!heapGS Σ, !cryptisGS Σ}.
 Notation iProp := (iProp Σ).
 
-Implicit Types (rl : role) (t kI kR nI nR sI sR kS : term).
+Implicit Types (rl : role) (t skI skR nI nR sI sR kS : term).
 Implicit Types (γ γa γb : gname) (ok : bool).
 Implicit Types (ts : nat) (T : gset term).
 Implicit Types (si : sess_info).
@@ -78,7 +78,8 @@ Lemma session_agree si1 si2 :
   si_key si1 = si_key si2 →
   si1 = si2.
 Proof.
-case: si1 si2 => [kI1 kR1 ga1 gb1 gab1] [kI2 kR2 ga2 gb2 gab2] /=.
+case: si1 si2
+  => [skI1 skR1 ga1 gb1 gab1] [skI2 skR2 ga2 gb2 gab2] /=.
 case/Spec.tag_inj => _.
 by case/Spec.of_list_inj => <- <- <- <- <-.
 Qed.
@@ -87,43 +88,117 @@ Definition compromised_session si : iProp :=
   compromised_key (si_init si) ∨
   compromised_key (si_resp si).
 
-Definition session_status si (failed : bool) : iProp := ∃ a,
-  ⌜si_init_share si = TExp (TInt 0) a⌝ ∗
-  term_meta a (nroot.@"failed") failed.
+Definition release_token share : iProp :=
+  term_token share (↑nroot.@"released").
 
-Lemma session_status_agree si failed1 failed2 :
-  session_status si failed1 -∗
-  session_status si failed2 -∗
-  ⌜failed1 = failed2⌝.
+Lemma release_tokenI share E :
+  ↑nroot.@"released" ⊆ E →
+  term_token share E -∗
+  release_token share ∗ term_token share (E ∖ ↑nroot.@"released").
 Proof.
-rewrite /session_status.
-iIntros "(%a1 & -> & #meta1) (%a2 & %e & #meta2)".
-move/TExp_injr: e => <-.
-by iApply (term_meta_agree with "meta1 meta2").
+iIntros "% ?"; by rewrite -term_token_difference.
 Qed.
 
-Definition msg2_pred kR m2 : iProp :=
+Definition released share : iProp :=
+  term_meta share (nroot.@"released") true.
+
+Lemma release share : release_token share ==∗ released share.
+Proof. by apply term_meta_set. Qed.
+
+Definition unreleased share : iProp :=
+  term_meta share (nroot.@"released") false.
+
+Lemma unrelease share : release_token share ==∗ unreleased share.
+Proof. by apply term_meta_set. Qed.
+
+Definition released_session si : iProp :=
+  released (si_init_share si) ∧ released (si_resp_share si).
+
+Lemma release_token_released_session si rl :
+  release_token (si_share_of rl si) -∗
+  released_session si -∗
+  False.
+Proof.
+iIntros "token [#init #resp]".
+iApply (term_meta_token with "token"); last by case: rl.
+by [].
+Qed.
+
+Lemma unreleased_released_session si rl :
+  unreleased (si_share_of rl si) -∗
+  released_session si -∗
+  False.
+Proof.
+iIntros "#un [#rI #rR]".
+iAssert (released (si_share_of rl si)) as "r"; first by case: rl.
+by iPoseProof (term_meta_agree with "r un") as "%".
+Qed.
+
+Definition key_secrecy si : iProp :=
+  □ (▷ released_session si → public (si_key si)) ∗
+  (compromised_session si ∨
+     □ (public (si_key si) → ▷ released_session si)).
+
+Lemma secret_key_secrecy si :
+  secret (si_init si) -∗
+  secret (si_resp si) -∗
+  sign_key (si_init si) -∗
+  sign_key (si_resp si) -∗
+  key_secrecy si -∗
+  ◇ □ (public (si_key si) ↔ ▷ released_session si).
+Proof.
+iIntros "sI sR #signI #signR [#? [#comp|#?]]"; eauto.
+iDestruct "comp" as "[comp|comp]".
+- by iDestruct (sign_secret_not_compromised_key with "sI [//] [//]")
+    as ">[]".
+- by iDestruct (sign_secret_not_compromised_key with "sR [//] [//]")
+    as ">[]".
+Qed.
+
+Lemma unreleased_key_secrecy rl si :
+  unreleased (si_share_of rl si) -∗
+  □ (public (si_key si) ↔ ▷ released_session si) -∗
+  □ (public (si_key si) ↔ ▷ False).
+Proof.
+iIntros "#un #s_k !>".
+iApply (bi.iff_trans _ (▷ released_session si)). iSplit => //.
+iSplit; last by iIntros ">[]".
+iIntros "#re !>".
+by iApply unreleased_released_session.
+Qed.
+
+Lemma release_token_key_secrecy rl si :
+  release_token (si_share_of rl si) -∗
+  □ (public (si_key si) ↔ ▷ released_session si) -∗
+  public (si_key si) -∗
+  ▷ False.
+Proof.
+iIntros "token #s_k #p_k".
+iPoseProof ("s_k" with "p_k") as "contra".
+iModIntro. by iApply (release_token_released_session with "token").
+Qed.
+
+Definition msg2_pred skR m2 : iProp :=
   ∃ ga b vkI,
-    let vkR := TKey Open kR in
+    let vkR := TKey Open skR in
     let gb := TExp (TInt 0) b in
     let gab := TExp ga b in
     let secret := Spec.of_list [vkI; vkR; ga; gb; gab] in
     let key := Spec.derive_key secret in
     ⌜m2 = Spec.of_list [ga; gb; vkI]⌝ ∗
-    (public b ↔ ▷ □ False) ∗
+    (public b ↔ ▷ (released ga ∧ released gb)) ∗
     (∀ t, dh_pred b t ↔ ▷ □ iso_dh_pred t).
 
 Definition msg3_pred kI m3 : iProp :=
-  ∃ a gb kR failed,
+  ∃ a gb kR,
     let vkI := TKey Open kI in
     let vkR := TKey Open kR in
     let ga := TExp (TInt 0) a in
     let gab := TExp gb a in
     let si := SessInfo kI kR ga gb gab in
     ⌜m3 = Spec.of_list [ga; gb; vkR]⌝ ∗
-    session_status si failed ∗
-    (◇ public (si_key si) ↔ ▷ ⌜failed⌝) ∗
-    (compromised_session si ∨ ⌜failed = false⌝).
+    (compromised_session si ∨
+     □ (public (si_key si) → ▷ released_session si)).
 
 Definition iso_dh_ctx : iProp :=
   seal_pred (N.@"m2") msg2_pred ∗
@@ -142,19 +217,18 @@ iMod (seal_pred_set (N.@"m3") msg3_pred with "token")
 iModIntro. by iSplit.
 Qed.
 
-Lemma public_dh_secret a b :
-  □ (public a ↔ ▷ □ False) -∗
+Lemma public_dh_secret a b (P : iProp ) :
+  □ (public a ↔ ▷ P) -∗
   □ (∀ t, dh_pred a t ↔ ▷ □ iso_dh_pred t) -∗
-  □ (public b ↔ ▷ □ False) -∗
+  □ (public b ↔ ▷ P) -∗
   □ (∀ t, dh_pred b t ↔ ▷ □ iso_dh_pred t) -∗
-  ◇ public (TExpN (TInt 0) [a; b]) ↔ ▷ False.
+  (public (TExpN (TInt 0) [a; b]) → ▷ P).
 Proof.
 iIntros "#s_a #pred_a #s_b #pred_b".
 rewrite public_TExp2_iff //; last by eauto.
-iSplit; last by iIntros ">[]".
-iIntros "> [[_ #p_b] | [[_ #p_a] | (_ & contra & _)]]".
-- by iDestruct ("s_b" with "p_b") as ">[]".
-- by iDestruct ("s_a" with "p_a") as ">[]".
+iIntros "[[_ #p_b] | [[_ #p_a] | (_ & contra & _)]]".
+- by iApply "s_b".
+- by iApply "s_a".
 iPoseProof ("pred_a" with "contra") as ">%contra".
 by rewrite /iso_dh_pred exps_TExpN /= in contra.
 Qed.
