store/connection_proofs.v
@@ -47,15 +47,12 @@ wp_apply (wp_initiator with "[//] [//] [//] [] []") => //.
 iIntros "%res resP".
 case: res=> [kS|] /=; wp_pures; last by iLeft; iFrame; eauto.
 iDestruct "resP"
-  as "(%si & %failed & % & %e_kR & <- &
-       #m_kS & #status & #s_kS & #s_kS' & #comp & token)".
+  as "(%si & % & %e_kR & <- & #m_kS & #s_kS & #comp & token)".
 case: e_kR => <-.
 wp_alloc ts as "ts". wp_pures.
 iRight. iModIntro. iExists _.  iSplit => //.
 iApply ("post" $! (ConnState si ts Init)). iFrame => /=.
 do !iSplit => //.
-iDestruct "comp" as "[fail|->]"; last by iRight.
-by eauto.
 Qed.
 
 Lemma wp_connection_listen N c kR :
@@ -85,8 +82,7 @@ iDestruct "resP"
 wp_pures.
 iRight. iModIntro. iExists _.  iSplit => //.
 iApply ("post" $! (ConnState si ts Resp)). iFrame => /=.
-do !iSplit => //; eauto.
-iDestruct "comp" as "[fail|[_ sess]]"; eauto.
+by do !iSplit => //; eauto.
 Qed.
 
 Lemma wp_connection_timestamp cs (n : nat) :
@@ -255,10 +251,11 @@ Definition handler_correct φ Φ cs handler n : iProp :=
     □ ∀ m, ▷ public m -∗
            □ ▷ session_failed_or cs (Ψ cs m) -∗
            wf_conn_state cs -∗
+           release_token (cs_share cs) -∗
            cs_ts cs ↦ #n -∗
            φ -∗
            WP (f : val) m {{ v,
-             ⌜v = NONEV⌝ ∗ cs_ts cs ↦ #n ∗ φ ∨
+             ⌜v = NONEV⌝ ∗ cs_ts cs ↦ #n ∗ release_token (cs_share cs) ∗ φ ∨
              ∃ r, ⌜v = SOMEV r⌝ ∗ Φ r }}
   }}%I.
 
@@ -266,21 +263,22 @@ Lemma wp_connection_select φ Φ (c : val) cs n (handlers : list (namespace * ex
   channel c -∗
   ([∗ list] handler ∈ handlers, handler_correct φ Φ cs handler n) -∗
   wf_conn_state cs -∗
+  release_token (cs_share cs) -∗
   cs_ts cs ↦ #n -∗
   φ -∗
   WP Connection.select c (repr cs) handlers {{ Φ }}.
 Proof.
 rewrite Connection.select_eq /Connection.select_def.
-iIntros "#chan_c wps #conn ts inv".
+iIntros "#chan_c wps #conn rel ts inv".
 wp_bind (Connection.make_handlers _).
 iApply (wp_wand with "[wps]").
 { iApply (wp_connection_make_handlers
-            (cs_ts cs ↦ #n ∗ φ) Φ (si_key cs)
+            (cs_ts cs ↦ #n ∗ release_token (cs_share cs) ∗ φ) Φ (si_key cs)
            with "[wps]").
   iApply (big_sepL_impl with "wps").
   iIntros "!> % %handler _ wp".
   iApply (wp_wand with "wp").
-  iIntros "%f #wp !> %m #p_m [ts inv]".
+  iIntros "%f #wp !> %m #p_m (ts & rel & inv)".
   iDestruct "wp" as "(%Ψ & #seal & #wp)".
   iAssert (minted m) as "#m_m".
   { rewrite public_minted minted_TSeal minted_tag.
@@ -291,9 +289,14 @@ iApply (wp_wand with "[wps]").
     iDestruct (public_TSealE with "[//] [//]") as "{p_m} [[p_key p_m]|p_m]".
     - iSplitR => //.
       iSpecialize ("s_key" with "p_key").
+      rewrite -bi.later_intuitionistically.
+      iDestruct "s_key" as "{p_key} >p_key".
       iDestruct "sess'" as "(%failed & #[meta failed] & _)".
       case: failed; last first.
-      { iModIntro. by iDestruct ("failed" with "s_key") as ">[]". }
+      { iDestruct ("failed" with "p_key") as "#contra".
+        iModIntro.
+        by iDestruct (release_token_released_session with "rel contra")
+          as "[]". }
       iIntros "!> !>". iLeft.
       by case: (cs_role cs); [iLeft|iRight]; iSplit.
     - iDestruct "p_m" as "[#p_m _]".
@@ -301,10 +304,10 @@ iApply (wp_wand with "[wps]").
       iDestruct "p_m" as "(%si & %e_kS & #sess'' & inv_m)".
       iSplit => //. rewrite swap_roleK (session_agree e_kS).
       by iApply "inv_m". }
-  iApply ("wp" with "p_m [//] conn ts inv"). }
+  iApply ("wp" with "p_m [//] conn rel ts inv"). }
 iIntros "% (%handlers' & -> & #Hhandlers')".
 wp_pures. wp_apply wp_connection_session_key => //. iIntros "_".
-wp_pures. iCombine "ts inv" as "I". iRevert "I". iApply wp_do_until.
+wp_pures. iCombine "ts rel inv" as "I". iRevert "I". iApply wp_do_until.
 iIntros "!> I". wp_pures. wp_bind (recv _). iApply wp_recv => //.
 iIntros "%m #p_m". wp_pures.
 wp_apply wp_key.
@@ -315,7 +318,7 @@ iApply (wp_connection_select_body' Φ with "[] [] [] I").
 - iApply (big_sepL_impl with "Hhandlers'").
   iIntros "!> %k %handler _ #Hhandler inv" => //.
   by iApply ("Hhandler" with "p_m inv").
-- iIntros "[??]". iLeft. by iFrame.
+- iIntros "(?&?&?)". iLeft. by iFrame.
 - iIntros "%r Hr". iRight. iExists r. by eauto.
 Qed.
 
@@ -326,32 +329,39 @@ Lemma wp_connection_recv N c cs n (f : val) φ Φ rl Ψ :
   wf_conn_state cs -∗
   □ (∀ m,
       cs_ts cs ↦ #n -∗
+      release_token (cs_share cs) -∗
       φ -∗
       public m -∗
       □ session_failed_or cs (Φ cs m) -∗
-      WP f m {{ v, ⌜v = NONEV⌝ ∗ cs_ts cs ↦ #n ∗ φ ∨
+      WP f m {{ v, ⌜v = NONEV⌝ ∗
+                   cs_ts cs ↦ #n ∗ release_token (cs_share cs) ∗ φ ∨
                    ∃ v', ⌜v = SOMEV v'⌝ ∗ Ψ v' }}) -∗
-  cs_ts cs ↦ #n -∗ φ -∗ WP Connection.recv N c (repr cs) f {{ Ψ }}.
+  cs_ts cs ↦ #n -∗ release_token (cs_share cs) -∗ φ -∗
+  WP Connection.recv N c (repr cs) f {{ Ψ }}.
 Proof.
-iIntros "#chan #pred %e_rl #conn #post ts inv".
+iIntros "#chan #pred %e_rl #conn #post ts rel inv".
 move/(f_equal swap_role): e_rl; rewrite swap_roleK => <- {rl}.
 iPoseProof "conn" as "((#minted_kS & #s_key & #sess) & #sess')".
 wp_lam; wp_pures.
 wp_apply wp_connection_session_key => //. iIntros "_".
-wp_pures. iCombine "ts inv" as "I". iRevert "I".
+wp_pures. iCombine "ts rel inv" as "I". iRevert "I".
 iApply wp_do_until.
-iIntros "!> (ts & inv)".
+iIntros "!> (ts & rel & inv)".
 wp_pure _ credit:"c".
 wp_pures. wp_apply wp_recv => //.
 iIntros "%m #p_m". wp_pures. wp_sdec m; wp_pures; last by iLeft; iFrame.
 iAssert (▷ □ (public m ∗ session_failed_or cs (Φ cs m)))%I
-  as "{p_m} p_m".
+  as "{p_m} #p_m".
 { iDestruct (public_TSealE with "[//] [//]") as "{p_m} [[p_key p_m]|p_m]".
   - iSplitR => //.
     iSpecialize ("s_key" with "p_key").
     iDestruct "sess'" as "(%failed & #[meta failed] & _)".
+    iDestruct "s_key" as "{p_key} >p_key".
     case: failed; last first.
-    { by iDestruct ("failed" with "s_key") as ">[]". }
+    { iDestruct ("failed" with "p_key") as "#contra".
+      iModIntro.
+      by iDestruct (release_token_released_session with "rel contra")
+        as "[]". }
     iIntros "!> !>". iLeft.
     by case: (cs_role cs); [iLeft|iRight]; iSplit.
   - iDestruct "p_m" as "[#p_m _]".
@@ -360,7 +370,7 @@ iAssert (▷ □ (public m ∗ session_failed_or cs (Φ cs m)))%I
     iSplit => //.
     rewrite swap_roleK (session_agree e_kS). by iApply "inv_m". }
 iMod (lc_fupd_elim_later with "c p_m") as "{p_m} [#p_m #inv_m]".
-by iApply ("post" with "ts inv").
+by iApply ("post" with "ts rel inv").
 Qed.
 
 Lemma wp_connection_close (c : val) cs n :
