store/server_proofs/close.v
@@ -44,7 +44,8 @@ iIntros "%e_rl #chan_c #ctx".
 iPoseProof (store_ctx_close with "ctx") as "?".
 iPoseProof (store_ctx_ack_close with "ctx") as "?".
 rewrite /handler_correct e_rl /=. wp_lam; wp_pures. iModIntro.
-iExists _. iSplit => //. iIntros "!> %m #p_m #inv_m #conn ts (server & db)".
+iExists _. iSplit => //.
+iIntros "!> %m #p_m #inv_m #conn rel ts (server & db)".
 wp_pures. wp_bind (Connection.timestamp _).
 iApply (wp_connection_timestamp with "ts").
 iIntros "!> ts". wp_pures.
